examples/hwmcc_checker/translation/aig_fmapsProgScript.sml
@@ -5,182 +5,9 @@ Theory aig_fmapsProg
 Ancestors
   aig_cert_encodeProg aig_to_cnf
 Libs
-  preamble ml_translatorLib
+  preamble ml_translatorLib MapProgLib
 
 val _ = translation_extends "aig_cert_encodeProg";
-
-(*----------------------------------------------------------------------*
-   general tooling for adding mlmap support for fmaps
- *----------------------------------------------------------------------*)
-
-Definition FMAP_TYPE_def:
-  FMAP_TYPE cmp a b f v =
-    ∃m. mlmap$map_ok m ∧ mlmap$to_fmap m = f ∧ MAP_TYPE a b m v ∧
-        mlmap$cmp_of m = cmp
-End
-
-Theorem MAP_TYPE_empty_IMP_FMAP_TYPE:
-  MAP_TYPE a b (mlmap$empty cmp) v ∧ TotOrd cmp ⇒
-  FMAP_TYPE cmp a b FEMPTY v
-Proof
-  rw [FMAP_TYPE_def]
-  \\ last_x_assum $ irule_at Any
-  \\ fs [mlmapTheory.empty_thm]
-QED
-
-Theorem IMP_FMAP_TYPE_FLOOKUP:
-  (MAP_TYPE b a --> b --> OPTION_TYPE a) mlmap$lookup v ⇒
-  (FMAP_TYPE cmp b a --> b --> OPTION_TYPE a) FLOOKUP v
-Proof
-  fs [ml_translatorTheory.Arrow_def,FMAP_TYPE_def,
-      ml_translatorTheory.AppReturns_def]
-  \\ rw [] \\ simp [GSYM (mlmapTheory.lookup_thm)]
-QED
-
-Theorem IMP_FMAP_TYPE_FUPDATE:
-  (MAP_TYPE b a --> (b:'a -> v -> bool) --> a --> MAP_TYPE b a) mlmap$insert v ⇒
-  (FMAP_TYPE cmp b a --> b --> a --> FMAP_TYPE cmp b a) fmap_update v
-Proof
-  fs [ml_translatorTheory.Arrow_def,FMAP_TYPE_def,
-      ml_translatorTheory.AppReturns_def] \\ rw []
-  \\ fs [fmap_update_def]
-  \\ last_x_assum drule \\ strip_tac
-  \\ first_x_assum $ qspec_then ‘refs’ strip_assume_tac \\ fs []
-  \\ first_x_assum $ irule_at Any \\ rw []
-  \\ last_x_assum drule \\ strip_tac
-  \\ first_x_assum $ qspec_then ‘refs’ strip_assume_tac \\ fs []
-  \\ first_x_assum $ irule_at Any \\ rw []
-  \\ last_x_assum drule \\ strip_tac
-  \\ first_x_assum $ qspec_then ‘refs’ strip_assume_tac \\ fs []
-  \\ first_x_assum $ irule_at Any \\ rw []
-  \\ first_x_assum $ irule_at Any \\ rw []
-  \\ metis_tac [mlmapTheory.insert_thm]
-QED
-
-Theorem IMP_FMAP_TYPE_DOMSUB:
-  (MAP_TYPE b a --> (b:'a -> v -> bool) --> MAP_TYPE b a) mlmap$delete v ⇒
-  (FMAP_TYPE cmp b a --> b --> FMAP_TYPE cmp b a) $\\ v
-Proof
-  fs [ml_translatorTheory.Arrow_def,FMAP_TYPE_def,
-      ml_translatorTheory.AppReturns_def] \\ rw []
-  \\ last_x_assum drule \\ strip_tac
-  \\ first_x_assum $ qspec_then ‘refs’ strip_assume_tac \\ fs []
-  \\ first_x_assum $ irule_at Any \\ rw []
-  \\ last_x_assum drule \\ strip_tac
-  \\ first_x_assum $ qspec_then ‘refs’ strip_assume_tac \\ fs []
-  \\ first_x_assum $ irule_at Any \\ rw []
-  \\ first_x_assum $ irule_at Any \\ rw []
-  \\ metis_tac [mlmapTheory.delete_thm]
-QED
-
-Theorem IMP_FMAP_TYPE_FUNION:
-  (MAP_TYPE b a --> MAP_TYPE b a --> MAP_TYPE b a) mlmap$union v ⇒
-  (FMAP_TYPE cmp b a --> FMAP_TYPE cmp b a --> FMAP_TYPE cmp b a) FUNION v
-Proof
-  fs [ml_translatorTheory.Arrow_def,FMAP_TYPE_def,
-      ml_translatorTheory.AppReturns_def] \\ rw []
-  \\ last_x_assum drule \\ strip_tac
-  \\ first_x_assum $ qspec_then ‘refs’ strip_assume_tac \\ fs []
-  \\ first_x_assum $ irule_at Any \\ rw []
-  \\ last_x_assum drule \\ strip_tac
-  \\ first_x_assum $ qspec_then ‘refs’ strip_assume_tac \\ fs []
-  \\ first_x_assum $ irule_at Any \\ rw []
-  \\ first_x_assum $ irule_at Any \\ rw []
-  \\ metis_tac [mlmapTheory.union_thm]
-QED
-
-Theorem IMP_FMAP_TYPE_ops:
-  MAP_TYPE (key:'k -> v -> bool) (a:'a -> v -> bool) (mlmap$empty cmp) v ∧ TotOrd cmp ⇒
-  FMAP_TYPE cmp key a FEMPTY v ∧
-  ((MAP_TYPE key a --> key --> OPTION_TYPE a) mlmap$lookup v1 ⇒
-   (FMAP_TYPE cmp key a --> key --> OPTION_TYPE a) FLOOKUP v1) ∧
-  ((MAP_TYPE key a --> key --> a --> MAP_TYPE key a) mlmap$insert v1 ⇒
-   (FMAP_TYPE cmp key a --> key --> a --> FMAP_TYPE cmp key a) fmap_update v1) ∧
-  ((MAP_TYPE key a --> key --> MAP_TYPE key a) mlmap$delete v1 ⇒
-   (FMAP_TYPE cmp key a --> key --> FMAP_TYPE cmp key a) $\\ v1) ∧
-  ((MAP_TYPE key a --> MAP_TYPE key a --> MAP_TYPE key a) mlmap$union v1 ⇒
-   (FMAP_TYPE cmp key a --> FMAP_TYPE cmp key a --> FMAP_TYPE cmp key a) FUNION v1)
-Proof
-  rw []
-  >- (irule MAP_TYPE_empty_IMP_FMAP_TYPE \\ simp [])
-  >- (irule IMP_FMAP_TYPE_FLOOKUP \\ simp [])
-  >- (irule IMP_FMAP_TYPE_FUPDATE \\ simp [])
-  >- (irule IMP_FMAP_TYPE_DOMSUB \\ simp [])
-  >- (irule IMP_FMAP_TYPE_FUNION \\ simp [])
-QED
-
-val mlmap_lookup_v_thm =
-  match ["MapProg"] “(_ --> _) mlmap$lookup _” |> hd |> snd |> #1;
-val mlmap_union_v_thm =
-  match ["MapProg"] “(_ --> _) mlmap$union _” |> hd |> snd |> #1
-val mlmap_delete_v_thm =
-  match ["MapProg"] “(_ --> _) mlmap$delete _” |> hd |> snd |> #1;
-val mlmap_insert_v_thm =
-  match ["MapProg"] “(_ --> _) mlmap$insert _” |> hd |> snd |> #1;
-
-fun add_fmap_for_cmp th = let
-  val cmp_tm = th |> concl |> rand
-  val _ = hol2deep cmp_tm handle UnableToTranslate _ =>
-          failwith "Ordering must the translated first"
-  fun find_name name i = let
-    val s = if i < 0 then name else name ^ "_" ^ int_to_string i
-    in
-      (if (Parse.Term [QUOTE (s ^ " :'a ")] |> is_const) then
-         find_name name (i+1)
-       else s)
-      handle HOL_ERR _ => find_name name (i+1)
-    end
-  val const_name = find_name "fempty" (0-1)
-  val tm = mlmapTheory.empty_def |> ISPEC cmp_tm |> concl |> dest_eq |> fst
-  val def_tm = mk_eq(mk_var(const_name,type_of tm), tm)
-  val def = new_definition(const_name ^ "_def", def_tm)
-  val empty_v_thm = translate def
-  val lem = CONJ (empty_v_thm |> REWRITE_RULE [def]) th
-  val ops_thm = MATCH_MP IMP_FMAP_TYPE_ops lem
-  val fempty_thm = ops_thm |> cj 1
-  (* empty + teach about type’*)
-  val res = fempty_thm |> concl |> rator
-  val fmap_ty = res |> rand |> type_of
-  val fmap_inv = res |> rator
-  val _ = add_type_inv fmap_inv fmap_ty
-  val _ = add_user_proved_v_thm fempty_thm
-  (* lookup *)
-  val th1 = cj 2 ops_thm
-  val th2 = mlmap_lookup_v_thm
-  val tm1 = th1 |> concl |> dest_imp |> fst |> rator |> rator
-  val tm2 = th2 |> concl |> rator |> rator
-  val (i1,i2) = match_term tm2 tm1
-  val th2a = INST i1 (INST_TYPE i2 th2)
-  val flookup_thm = MATCH_MP th1 th2a
-  val _ = add_user_proved_v_thm flookup_thm
-  (* delete *)
-  val th1 = cj 4 ops_thm
-  val th2 = mlmap_delete_v_thm
-  val tm1 = th1 |> concl |> dest_imp |> fst |> rator |> rator
-  val tm2 = th2 |> concl |> rator |> rator
-  val (i1,i2) = match_term tm2 tm1
-  val th2a = INST i1 (INST_TYPE i2 th2)
-  val domsub_thm = MATCH_MP th1 th2a
-  val _ = add_user_proved_v_thm domsub_thm
-  (* update *)
-  val th1 = cj 3 ops_thm
-  val th2 = mlmap_insert_v_thm
-  val tm1 = th1 |> concl |> dest_imp |> fst |> rator |> rator
-  val tm2 = th2 |> concl |> rator |> rator
-  val (i1,i2) = match_term tm2 tm1
-  val th2a = INST i1 (INST_TYPE i2 th2)
-  val fmap_update_thm = MATCH_MP th1 th2a
-  val _ = add_user_proved_v_thm fmap_update_thm
-  (* union *)
-  val th1 = cj 5 ops_thm
-  val th2 = mlmap_union_v_thm
-  val tm1 = th1 |> concl |> dest_imp |> fst |> rator |> rator
-  val tm2 = th2 |> concl |> rator |> rator
-  val (i1,i2) = match_term tm2 tm1
-  val th2a = INST i1 (INST_TYPE i2 th2)
-  val funion_thm = MATCH_MP th1 th2a
-  val _ = add_user_proved_v_thm funion_thm
-  in () end;
 
 (*----------------------------------------------------------------------*
    specific types to target
@@ -197,50 +24,17 @@ Type ty6[local] = “:((num + num) iext + (num + num) iext) iext”;
    ty1
  *----------------------------------------------------------------------*)
 
-Definition num_cmp_def:
-  num_cmp n1 (n2:num) =
-    if n1 < n2 then LESS else
-    if n2 < n1 then GREATER else EQUAL
-End
-
 val _ = translate num_cmp_def;
 
 Theorem TotOrd_ty1:
   TotOrd (num_cmp : ty1 -> ty1 -> ordering)
 Proof
-  fs [totoTheory.TotOrd, num_cmp_def, CaseEq"bool"]
+  rewrite_tac [TotOrd_num_cmp]
 QED
 
 (*----------------------------------------------------------------------*
    ty2
  *----------------------------------------------------------------------*)
-
-Definition sum_cmp_def:
-  sum_cmp c1 c2 x1 x2 =
-    case x1 of
-    | INL n1 =>
-        (case x2 of
-         | INL n2 => c1 n1 n2
-         | INR _ => LESS)
-    | INR n1 =>
-        (case x2 of
-         | INL _ => GREATER
-         | INR n2 => c2 n1 n2)
-End
-
-Theorem sum_forall:
-  (∀x. P x) ⇔ (∀y. P (INL y)) ∧ (∀y. P (INR y))
-Proof
-  eq_tac \\ rw [] \\ simp [] \\ Cases_on ‘x’ \\ fs []
-QED
-
-Theorem TotOrd_sum:
-  TotOrd c1 ∧ TotOrd c2 ⇒
-  TotOrd (sum_cmp c1 c2)
-Proof
-  fs [totoTheory.TotOrd, sum_cmp_def, AllCaseEqs(), sum_forall]
-  \\ simp [SF DNF_ss, PULL_EXISTS] \\ rw [] \\ res_tac
-QED
 
 Definition num_sum_num_cmp_def:
   num_sum_num_cmp = sum_cmp num_cmp num_cmp
